\documentclass[a4paper, 11pt]{article}
\usepackage{amssymb}
\usepackage{enumitem}
\usepackage{fullpage}

\newlist{myEnumerate}{enumerate}{9}
\setlist[myEnumerate,1]{label=\arabic*.}
\setlist[myEnumerate,2]{label=(\alph*)}
\setlist[myEnumerate,3]{label=\roman*.}


\begin{document}

\noindent
\large\textbf{Assignment 4} \hfill \textbf{LE, Nhat Hung} \\
\normalsize MATH 240 \hfill \today

\begin{myEnumerate}
	\item
	
    \textbf{Division algorithm:}
    $$
    \forall a, b \in \mathbb{Z} \textnormal{ } (b \neq 0),
    \left\{
    	\begin{array}{ll}
        	a = qb + r \\
        	0 \leq r < |b|
    	\end{array}
	\right. \textnormal{with } q,r \in \mathbb{Z}
    $$
    
    \textbf{Case of $a = 0,$ $b \neq 0:$} $q,r = 0$
    
    \textbf{Case of $a, b < 0:$} \\
    Having proven the algorithm for $a, b > 0$, we know $-a = q(-b) + r$.
    
    \(
    \begin{array}{ll}
    	-a = q(-b) + r & \Rightarrow a = qb - r \\
        			   & \Rightarrow a = qb + b - b - r \\
                       & \Rightarrow a = (q + 1)b - b - r \\
                       & \Rightarrow
        \left\{
    		\begin{array}{ll}
        		a = q'b + r' \\
        		q' = q + 1, \textnormal{ } r' = -b - r \\
                0 \leq |b| - r < |b|
    		\end{array}
		\right. \\
        			  & \Rightarrow
        \left\{
    		\begin{array}{ll}
        		a = q'b + r' \\
        		0 \leq -b - r < |b|
    		\end{array}
		\right. \\
        			  & \Rightarrow
        \left\{
    		\begin{array}{ll}
        		a = q'b + r' \\
        		0 \leq r' < |b|
    		\end{array}
		\right.
    \end{array} \\ \)
    
    \textbf{Case of $a < 0,$ $b > 0:$}
    
    \(
    \begin{array}{ll}
    	-a = qb + r & \Rightarrow a = -qb - r \\
        			& \Rightarrow a = -qb - b + b - r \\
                    & \Rightarrow a = -(q + 1)b + b - r \\
                    & \Rightarrow 
        \left\{
    		\begin{array}{ll}
        		a = q'b + r' \\
        		q' = -(q + 1), \textnormal{ } r' = b - r \\
                0 \leq b - r < |b|
    		\end{array}
		\right. \\
        			& \Rightarrow 
        \left\{
    		\begin{array}{ll}
        		a = q'b + r' \\
                0 \leq r' < |b|
    		\end{array}
		\right.
    \end{array} \\ \)

	\textbf{Case of $a > 0,$ $b < 0:$}
    
    \(
    \begin{array}{ll}
    	a = q(-b) + r & \Rightarrow a = -qb + r \\
                      & \Rightarrow 
        \left\{
    		\begin{array}{ll}
        		a = q'b + r \\
        		q' = -q \\
                0 \leq r < |b|
    		\end{array}
		\right. \\
        			& \Rightarrow 
        \left\{
    		\begin{array}{ll}
        		a = q'b + r \\
                0 \leq r < |b|
    		\end{array}
		\right.
    \end{array} \\ \)
    
	\item
	\begin{myEnumerate}
    	\item
        \( \\
        \begin{array}{lllll}
        	2018 & = & 8 \cdot 240 & + & 98 \\
        	240  & = & 2 \cdot 98  & + & 44 \\
            98   & = & 2 \cdot 44  & + & 10 \\
            44   & = & 4 \cdot 10  & + & 4 \\
            10   & = & 2 \cdot 4   & + & 2 \\
            4    & = & 2 \cdot 2
    	\end{array} \\ \)
        
        $gcd(2018, 240) = 2$ 
        
        \(
        \begin{array}{lll}
        	10 = 2 \cdot 4 + 2 & \Rightarrow 10 - 2 \cdot 4 = 2 \\
            				   & \Rightarrow (98 - 2 \cdot 44) - 2(44 - 4 \cdot 10) = 2 \\
            				   & \Rightarrow 98 - 4 \cdot 44 + 8 \cdot 10 = 2 \\
                               & \Rightarrow 2018 - 8 \cdot 240 - 4(240 - 2 \cdot 98) + 8(98 - 2 \cdot 44) = 2 \\
                               & \Rightarrow 2018 - 12 \cdot 240 + 16 \cdot 98 - 16 \cdot 44 = 2 \\
                               & \Rightarrow 2018 - 12 \cdot 240 + 16(2018 - 8 \cdot 240) - 16(240 - 2 \cdot 98) = 2 \\
                               & \Rightarrow 17 \cdot 2018 - 156 \cdot 240 + 32 \cdot 98 = 2 \\
                               & \Rightarrow 17 \cdot 2018 - 156 \cdot 240 + 32(2018 - 8 \cdot 240) = 2 \\
                               & \Rightarrow 49 \cdot 2018 - 412 \cdot 240 = 2
        \end{array} \\\\ \)
        
        \item
        $gcd(a,b) = 1 \Rightarrow la + mb = 1, \textnormal{ } l,b \in \mathbb{Z}$ \\
        \( \\
        \begin{array}{lll}
       		\left\{
    			\begin{array}{l}
        			la(k^{2} - 1) = kl(b + ka) - klb - la \\
        			mb(k^{2} - 1) = km(a + kb) - kma - mb
    			\end{array}
			\right.
        & \Rightarrow & (k^{2} - 1)(la + mb) = kl(a + kb) + km(b + ka) \\
        && 									   - klb - la - kma - mb \\
        & \Rightarrow & (k^{2} - 1) \cdot 1 = kl(a + kb) + km(b + ka) \\
        &&									  - l(a + kb) - m(b + ka) \\
        & \Rightarrow & (k^{2} - 1) = (kl - m)(a + kb) + (km - l)(b + ka) \\
        & \Rightarrow &
        \left\{
    			\begin{array}{l}
        			d \mid (k^{2} - 1) \\
        			d = gcd(a + kb, b + ka)
    			\end{array}
			\right.
        \end{array} \)
        
        \item
        \( \\
        \begin{array}{ll}
        	\left\{
    			\begin{array}{l}
        			p $ prime $ \\
        			p \mid n \\
                    p \nmid m
    			\end{array}
			\right.
            & \Rightarrow 
            \left\{
    			\begin{array}{l}
        			gcd(p, m) = 1 \\
        			p \mid (m \cdot \frac{n}{m})
    			\end{array}
			\right.\\
            & \Rightarrow p \mid \frac{n}{m}
        \end{array} \\ \)

    \end{myEnumerate}

    \item
    \begin{myEnumerate}
    	\item
        \( \\
        \begin{array}{ll|ll}
            	ka \equiv kb \textnormal{ (mod $kn$)} &  \Rightarrow kn|(ka - kb)
                & a \equiv b \textnormal{ (mod $n$)}  &  \Rightarrow n|(a - b) \\
                									  &  \Rightarrow ka - kb = l(kn), \textnormal{ } l\in \mathbb{Z}
                                                      && \Rightarrow a - b = mn, \textnormal{ } m\in \mathbb{Z} \\
                									  &  \Rightarrow a - b = ln 
                                                      && \Rightarrow ka - kb = m(kn) \\
                									  &  \Rightarrow n|(a - b) 
                                                      && \Rightarrow kn|(ka - kb) \\
                									  &  \Rightarrow a \equiv b \textnormal{ (mod n)}
                                                      && \Rightarrow ka \equiv kb \textnormal{ (mod kn)}
        \end{array} \\ \)
        
        Thus, $ka \equiv kb $ $ ($mod $ kn) \Leftrightarrow a \equiv b$ (mod $n$) \\
        
        \item
        $a \equiv b $ $ ($mod $n) \Rightarrow a - b = kn, $ $k \in \mathbb{Z}$ \\
        Let $c = gcd(a,n), $ $ d = gcd(b,n)$. \\
        \( \\
        \begin{array}{ll}
        	a - b = kn & \Rightarrow \frac{a}{c} - \frac{n}{c}k = \frac{b}{c} \\
            		   & \Rightarrow c|b \\
                       & \Rightarrow c \leq d
        \end{array} \\ \)
        
        Similarly, $d|a$ and $d \leq c$. \\
        Thus, c = d, or $gcd(a,n)=gcd(b,n)$. \\
        
        \item
        \( \\
        \begin{array}{ll}
        	1806 \equiv 4 $ (mod $17$)$ & \Rightarrow 1806^{2} \equiv 16 \equiv -1 $ (mod $17$)$ \\
            							  & \Rightarrow (1806^{2})^{3118} \equiv (-1)^{3118} $ (mod $17$)$ \\
                                          & \Rightarrow 1806^{6236} \equiv 1 $ (mod $17$)$
        \end{array} \)
        
    \end{myEnumerate}

\end{myEnumerate}

\end{document}
